theories/lang/cpp/logic/wp.v
@@ -1090,3 +1090,4 @@ End WPE.
 
 Export WPE.
 Export stdpp.coPset.
+Export cqp.
